Good progress on Flag-Based Effect Polymorphism variant

state/Witnessable.fst
@@ -17,6 +17,7 @@ noeq type linkedList (a: Type0) : Type0 =
 
 class witnessable (t:Type) = {
   satisfy : t -> lheap -> ref_lheap_pred -> Type0;
+  satisfy_refinement : t -> (#a:Type -> #rel:_ -> mref a rel -> Type0) -> Type0;
 
   satisfy_monotonic : x:t -> pred:ref_lheap_pred -> h0:lheap -> h1:lheap -> Lemma (
     h0 `lheap_rel` h1 /\ satisfy x h0 pred ==> satisfy x h1 pred);
@@ -28,6 +29,7 @@ class witnessable (t:Type) = {
 
 instance witnessable_ref (t:Type) {| c:witnessable t |} : witnessable (ref t) = {
   satisfy = (fun x h pred -> pred x h);
+  satisfy_refinement = (fun x pred -> pred x);
   satisfy_monotonic = (fun x pred h0 h1 -> ());
   witness = (fun x pred ->
     mst_witness (pred x);
@@ -36,12 +38,14 @@ instance witnessable_ref (t:Type) {| c:witnessable t |} : witnessable (ref t) = 
 
 instance witnessable_unit : witnessable unit = {
   satisfy = (fun _ _ _ -> True);
+  satisfy_refinement = (fun _ _ -> True);
   satisfy_monotonic = (fun _ _ _ _ -> ());
   witness = (fun _ _ -> (fun () -> ()));
 }
 
 instance witnessable_int : witnessable int = {
   satisfy = (fun _ _ _ -> True);
+  satisfy_refinement = (fun _ _ -> True);
   satisfy_monotonic = (fun _ _ _ _ -> ());
   witness = (fun _ _ -> (fun () -> ()));
 }
@@ -52,12 +56,14 @@ instance witnessable_arrow
   (post:t1 -> lheap -> t2 -> lheap -> Type0) // TODO: one cannot have pre-post depending on outside things.
 : witnessable (x:t1 -> ST t2 (pre x) (post x)) = {
   satisfy = (fun _ _ _ -> True);
+  satisfy_refinement = (fun _ _ -> True);
   satisfy_monotonic = (fun _ _ _ _ -> ());
   witness = (fun _ _ -> (fun () -> ()));
 }
 
 instance witnessable_pair (t1:Type) (t2:Type) {| c1:witnessable t1 |} {| c2:witnessable t2 |} : witnessable (t1 * t2) = {
   satisfy = (fun (x1, x2) h pred -> c1.satisfy x1 h pred /\ c2.satisfy x2 h pred);
+  satisfy_refinement = (fun (x1, x2) pred -> c1.satisfy_refinement x1 pred /\ c2.satisfy_refinement x2 pred);
   satisfy_monotonic = (fun (x1, x2) pred h0 h1 -> 
     c1.satisfy_monotonic x1 pred h0 h1;
     c2.satisfy_monotonic x2 pred h0 h1);
@@ -72,6 +78,10 @@ instance witnessable_sum (t1:Type) (t2:Type) {| c1:witnessable t1 |} {| c2:witne
     match x with
     | Inl x1 -> c1.satisfy x1 h pred
     | Inr x2 -> c2.satisfy x2 h pred);
+  satisfy_refinement = (fun x pred ->
+    match x with
+    | Inl x1 -> c1.satisfy_refinement x1 pred
+    | Inr x2 -> c2.satisfy_refinement x2 pred);
   satisfy_monotonic = (fun x pred h0 h1 ->
     match x with
     | Inl x1 -> c1.satisfy_monotonic x1 pred h0 h1
@@ -87,6 +97,12 @@ instance witnessable_llist (t:Type) {| c:witnessable t |} : witnessable (linkedL
     match l with
     | Nil -> True
     | Cons x xsref -> c.satisfy x h pred /\ pred xsref h
+  );
+
+  satisfy_refinement = (fun l pred ->
+    match l with
+    | Nil -> True
+    | Cons x xsref -> c.satisfy_refinement x pred /\ pred xsref
   );
 
   satisfy_monotonic = (fun l pred h0 h1 ->
@@ -107,6 +123,7 @@ instance witnessable_llist (t:Type) {| c:witnessable t |} : witnessable (linkedL
 
 instance witnessable_univ_raise (t:Type u#a) {| c:witnessable t |} : witnessable (raise_t u#a u#b t) = {
   satisfy = (fun x -> c.satisfy (downgrade_val x));
+  satisfy_refinement = (fun x -> c.satisfy_refinement (downgrade_val x));
   satisfy_monotonic = (fun x -> c.satisfy_monotonic (downgrade_val x));
   witness = (fun x -> c.witness (downgrade_val x));
 }
