state/FlagBasedEffPoly.fst
@@ -1,0 +1,130 @@
+module FlagBasedEffPoly
+
+open Labeled.Monotonic.Heap
+open Labeled.MST
+open Witnessable
+open TargetLang
+open STLC 
+
+(** for the very general idea, look into experiments/FlagBasedEffPoly.fst **)
+
+type fo_ctx =
+  // fl:erased tflag -> (** we don't have flag yets for ST **)
+  #inv:(lheap -> Type0) -> (** invariant on the heap **)
+  #prref: (#a:Type -> #rel:_ -> mref a rel -> Type0) ->
+  (** ^ if this predicate would be also over heaps, then the contexts needs witness&recall in HO settings **)
+  read :  ((#t:typ0) -> x:ref (elab_typ0 t) -> 
+            ST (elab_typ0 t) 
+              (requires (fun h0 -> inv h0 /\ (elab_typ0_tc (TRef t)).satisfy_refinement x prref))
+              (ensures  (fun h0 r h1 -> h0 == h1 /\ sel h1 x == r /\ (elab_typ0_tc t).satisfy_refinement r prref))) ->
+  write : ((#t:typ0) -> x:ref (elab_typ0 t) -> v:(elab_typ0 t) -> 
+            ST unit
+              (requires (fun h0 -> inv h0 /\ (elab_typ0_tc (TRef t)).satisfy_refinement x prref /\ (elab_typ0_tc t).satisfy_refinement v prref))
+              (ensures  (fun h0 _ h1 -> inv h1 /\ sel h1 x == v /\ modifies_only_label Low h0 h1 /\ modifies_classification Set.empty h0 h1))) ->
+  alloc : ((#t:typ0) -> init:(elab_typ0 t) -> 
+            ST (ref (elab_typ0 t)) 
+              (requires (fun h0 -> inv h0 /\ (elab_typ0_tc t).satisfy_refinement init prref))
+              (ensures  (fun h0 r h1 -> inv h1 /\ sel h1 r == init /\ (elab_typ0_tc (TRef t)).satisfy_refinement r prref /\ modifies_only_label Low h0 h1 /\ modifies_classification Set.empty h0 h1))) ->
+  (** type of the context: *)
+  unit -> ST unit (inv) (fun h0 _ h1 -> inv h1 /\ modifies_only_label Low h0 h1 /\ modifies_classification Set.empty h0 h1)
+
+(** Checking if there exists read, write, alloc so that we can instantiate the polymorphic context **)
+
+unfold
+let is_low_pred' r : pred:heap_predicate{stable pred} = (* F* being silly. There is an SMTPat on is_low_pred_stable **)
+  let pred = is_low_pred r in
+  is_low_pred_stable r;
+  pred
+ 
+let check_instantiating_the_context (ctx:fo_ctx) = 
+  ctx
+    #(fun h -> inv_low_contains h)
+    #(fun r -> witnessed (contains_pred r) /\ witnessed (is_low_pred' r)) 
+    (fun #t r -> (* READ *)
+      let h0 = get () in
+      mst_recall (contains_pred r); 
+      mst_recall (is_low_pred r);
+      let v = read r in
+      assert ((elab_typ0_tc t).satisfy v h0 contains_pred);
+      assert ((elab_typ0_tc t).satisfy v h0 is_low_pred);
+      assume ((elab_typ0_tc t).satisfy_refinement v (fun r' -> witnessed (contains_pred r') /\ witnessed (is_low_pred' r'))); (** one can create witnesses using the previous assertions **)
+      v) 
+    (fun #t r v -> (* WRITE *)
+      mst_recall (contains_pred r); 
+      mst_recall (is_low_pred r); 
+      let h0 = get () in
+      assume (shallowly_contained_low v #(elab_typ0_tc t) h0); (** one has to recall on v. a method on witnessable, that given a `witnessed pred`, returns a `satisfy pred`. **)
+      elab_write r v)
+    (fun #t init -> (* ALLOC *)
+      let h0 = get () in
+      assume (shallowly_contained_low init #(elab_typ0_tc t) h0); (** one has to recall on init **)
+      let r = elab_alloc init in 
+      mst_witness (contains_pred r); mst_witness (is_low_pred r);
+      r)
+
+
+(** TODO: Can the context easily/automatically work with the pre- and post-conditions? **)
+
+val ctx_update_ref_test : fo_ctx
+let ctx_update_ref_test my_read my_write my_alloc () =
+  let x = my_alloc 5 in
+  let y = my_read x in
+  my_write #TNat x (y+1);
+  ()
+
+type ho_ctx1 = (** only the type of the context is different **)
+  // fl:erased tflag ->
+  #inv:(lheap -> Type0) -> (** invariant on the heap **)
+  #prref: (#a:Type -> #rel:_ -> mref a rel -> Type0) ->
+  read :  ((#t:typ0) -> x:ref (elab_typ0 t) -> 
+            ST (elab_typ0 t) 
+              (requires (fun h0 -> inv h0 /\ (elab_typ0_tc (TRef t)).satisfy_refinement x prref))
+              (ensures  (fun h0 r h1 -> h0 == h1 /\ sel h1 x == r /\ (elab_typ0_tc t).satisfy_refinement r prref))) ->
+  write : ((#t:typ0) -> x:ref (elab_typ0 t) -> v:(elab_typ0 t) -> 
+            ST unit
+              (requires (fun h0 -> inv h0 /\ (elab_typ0_tc (TRef t)).satisfy_refinement x prref /\ (elab_typ0_tc t).satisfy_refinement v prref))
+              (ensures  (fun h0 _ h1 -> inv h1 /\ sel h1 x == v /\ modifies_only_label Low h0 h1 /\ modifies_classification Set.empty h0 h1))) ->
+  alloc : ((#t:typ0) -> init:(elab_typ0 t) -> 
+            ST (ref (elab_typ0 t)) 
+              (requires (fun h0 -> inv h0 /\ (elab_typ0_tc t).satisfy_refinement init prref))
+              (ensures  (fun h0 r h1 -> inv h1 /\ sel h1 r == init /\ (elab_typ0_tc (TRef t)).satisfy_refinement r prref /\ modifies_only_label Low h0 h1 /\ modifies_classification Set.empty h0 h1))) ->
+  (** type of the context: *)
+  rr:ref (ref int) -> ST (r:ref int -> ST unit (fun h0 -> inv h0 /\ satisfy_refinement r prref) (fun h0 _ h1 -> inv h1 /\ modifies_only_label Low h0 h1 /\ modifies_classification Set.empty h0 h1))
+    (requires (fun h0 -> inv h0 /\ satisfy_refinement rr prref))
+    (ensures  (fun h0 _ h1 -> inv h1 /\ modifies_only_label Low h0 h1 /\ modifies_classification Set.empty h0 h1))
+
+val ctx_update_multiple_refs_test : ho_ctx1
+let ctx_update_multiple_refs_test my_read my_write my_alloc x y =
+  let ix = my_read #(TRef TNat) x in
+  my_write #(TRef TNat) x y;
+  my_write #TNat y ((my_read #TNat y) + 5);
+  ()
+
+
+type ho_ctx2 =
+  // fl:erased tflag ->
+  #inv:(lheap -> Type0) -> (** invariant on the heap **)
+  #prref: (#a:Type -> #rel:_ -> mref a rel -> Type0) ->
+  read :  ((#t:typ0) -> x:ref (elab_typ0 t) -> 
+            ST (elab_typ0 t) 
+              (requires (fun h0 -> inv h0 /\ (elab_typ0_tc (TRef t)).satisfy_refinement x prref))
+              (ensures  (fun h0 r h1 -> h0 == h1 /\ sel h1 x == r /\ (elab_typ0_tc t).satisfy_refinement r prref))) ->
+  write : ((#t:typ0) -> x:ref (elab_typ0 t) -> v:(elab_typ0 t) -> 
+            ST unit
+              (requires (fun h0 -> inv h0 /\ (elab_typ0_tc (TRef t)).satisfy_refinement x prref /\ (elab_typ0_tc t).satisfy_refinement v prref))
+              (ensures  (fun h0 _ h1 -> inv h1 /\ sel h1 x == v /\ modifies_only_label Low h0 h1 /\ modifies_classification Set.empty h0 h1))) ->
+  alloc : ((#t:typ0) -> init:(elab_typ0 t) -> 
+            ST (ref (elab_typ0 t)) 
+              (requires (fun h0 -> inv h0 /\ (elab_typ0_tc t).satisfy_refinement init prref))
+              (ensures  (fun h0 r h1 -> inv h1 /\ sel h1 r == init /\ (elab_typ0_tc (TRef t)).satisfy_refinement r prref /\ modifies_only_label Low h0 h1 /\ modifies_classification Set.empty h0 h1))) ->
+  (** type of the context: *)
+  rr:ref ((ref int) * (ref int)) -> ST (unit -> ST unit (fun h0 -> inv h0) (fun h0 _ h1 -> inv h1 /\ modifies_only_label Low h0 h1 /\ modifies_classification Set.empty h0 h1))
+    (requires (fun h0 -> inv h0 /\ satisfy_refinement rr prref))
+    (ensures  (fun h0 _ h1 -> inv h1 /\ modifies_only_label Low h0 h1 /\ modifies_classification Set.empty h0 h1))
+
+val ctx_HO_test1 : ho_ctx2
+let ctx_HO_test1 #inv #prref my_read my_write my_alloc rr =
+  let (x', x'') = my_read #(TPair (TRef TNat) (TRef TNat)) rr in
+  my_write #(TPair (TRef TNat) (TRef TNat)) rr (x', x');
+  (fun _ ->
+    my_write #(TPair (TRef TNat) (TRef TNat)) rr (x', x''))
